Merge Joinable/ files

Instances/Joinable.v
@@ -1,7 +1,75 @@
 Require Import Classes.Joinable.
 Require Import Classes.PreorderedSet.
+Require Import Coq.Logic.FunctionalExtensionality.
+Require Import Instances.Preorder.AbstractStore.
 Require Import Instances.Preorder.Result.
+Require Import Instances.Preorder.Unit.
+Require Import Language.Statements.
 Require Import Types.Result.
+Require Import Types.Stores.
+
+Definition abstract_store_join
+  (ast1 ast2 : abstract_store) : abstract_store :=
+  fun x => VTop.
+
+Lemma abstract_store_join_comm : forall ast1 ast2,
+  abstract_store_join ast1 ast2 = abstract_store_join ast2 ast1.
+Proof. 
+  intros. unfold abstract_store_join. apply functional_extensionality.
+  intros. reflexivity. 
+Qed.
+
+Lemma abstract_store_join_assoc : forall ast1 ast2 ast3,
+  abstract_store_join ast1 (abstract_store_join ast2 ast3) =
+  abstract_store_join (abstract_store_join ast1 ast2) ast3.
+Proof. 
+  intros. unfold abstract_store_join. apply functional_extensionality.
+  intros. reflexivity.
+Qed.
+
+Lemma abstract_store_join_upperbound_left :
+    forall s s', preorder s (abstract_store_join s s').
+Proof.
+  simpl. unfold abstract_store_join. constructor.
+  intro x. constructor.
+Qed.
+
+Lemma abstract_store_join_upperbound_right : 
+  forall s s', preorder s' (abstract_store_join s s').
+Proof.
+  simpl. unfold abstract_store_join. constructor.
+  intro x. constructor.
+Qed.
+
+Global Instance abstract_store_joinable : Joinable abstract_store := {
+  join_op := abstract_store_join;
+  join_upper_bound_left := abstract_store_join_upperbound_left;
+  join_upper_bound_right := abstract_store_join_upperbound_right;
+}.
+
+
+Definition unit_join : unit -> unit -> unit :=
+    fun _ _ => tt.
+
+Lemma unit_join_upperbound_left : forall (u u' : unit),
+  preorder u (unit_join u u').
+Proof.
+  intros. destruct u, u'. unfold unit_join. apply preorder_refl.
+Qed.
+
+Lemma unit_join_upperbound_right : forall (u u' : unit),
+  preorder u' (unit_join u u').
+Proof.
+  intros. destruct u, u'. unfold unit_join. apply preorder_refl.
+Qed.
+
+Global Instance unit_joinable : Joinable unit :=
+{
+  join_op := unit_join;
+  join_upper_bound_left := unit_join_upperbound_left;
+  join_upper_bound_right := unit_join_upperbound_right
+}.
+
 
 Section result_joinable.
 Context {A S : Type} `{Joinable A, Joinable S}.
