Instances/IsBool/AbstractBoolean.v
@@ -2,7 +2,7 @@ Require Import Classes.IsBool.
 Require Import Classes.Joinable.
 Require Import Classes.Monad.
 Require Import Instances.Except.AbstractException.
-Require Import Instances.Joinable.Unit.
+Require Import Instances.Joinable.
 Require Import Language.Statements.
 Require Import Types.AbstractBool.
 Require Import Types.Result.
